DiskLog: checkpoint progress
It's not possible to automate the proofs as much as I would like right now
because the tactics fairly randomly trigger Coq anomalies. Thus, I've
bashed my way through most of the proofs, but hopefully I'll be able to
clean things up a bit.

src/DiskLog.v
@@ -192,6 +192,7 @@ Module DISKLOG.
       exists rest rest2,
       (LogDescriptor xp) |-> (descriptor_to_valu (map fst l ++ rest), [descriptor_to_valu (map fst l ++ rest2)]) *
       [[ @Rec.well_formed descriptor_type (map fst l ++ rest) ]] *
+      [[ @Rec.well_formed descriptor_type (map fst l ++ rest2) ]] *
       array (LogData xp) (synced_list (map snd l)) $1 *
       avail_region (LogData xp ^+ $ (length l))
                          (wordToNat (LogLen xp) - length l))%pred.
@@ -278,6 +279,11 @@ Module DISKLOG.
   Lemma combine_one: forall A B (a: A) (b: B), [(a, b)] = List.combine [a] [b].
   Proof.
     intros; auto.
+  Qed.
+
+  Lemma cons_combine : forall A B (a: A) (b: B) x y,
+    (a, b) :: List.combine x y = List.combine (a :: x) (b :: y).
+    trivial.
   Qed.
 
   Definition emp_star_r' : forall V AT AEQ P, P * (emp (V:=V) (AT:=AT) (AEQ:=AEQ)) =p=> P.
@@ -445,7 +451,7 @@ Module DISKLOG.
   Qed.
 
   Hint Rewrite firstn_combine_comm skipn_combine_comm selN_combine map_fst_combine map_snd_combine
-    removeN_combine List.combine_split combine_nth combine_one updN_0_skip_1 skipn_selN : lists.
+    removeN_combine List.combine_split combine_nth combine_one cons_combine updN_0_skip_1 skipn_selN : lists.
   Hint Rewrite <- combine_updN combine_upd combine_app : lists.
 
   Ltac split_pair_list_vars :=
@@ -639,56 +645,61 @@ Module DISKLOG.
     Rof ^(cs);
     rx ^(cs).
 
-(*
-  Definition extend_sync T xp (mscs : memstate_cachestate) rx : prog T :=
-    let '^(ms, cs) := mscs in
+  Definition extend_sync T xp (cs: cachestate) (old: log_contents) (oldlen: addr) (new: log_contents) rx : prog T :=
     cs <- BUFCACHE.sync (LogDescriptor xp) cs;
-    let^ (cs) <- For i < $ (Map.cardinal ms)
+    let^ (cs) <- For i < $ (length new)
     Ghost [ crash F ]
     Loopvar [ cs ]
     Continuation lrx
     Invariant
       exists d', BUFCACHE.rep cs d' *
       [[ (F
-          * exists rest, (LogDescriptor xp) |=> descriptor_to_valu (map fst (Map.elements ms) ++ rest)
-          * [[ @Rec.well_formed descriptor_type (map fst (Map.elements ms) ++ rest) ]]
-          * array (LogData xp) (firstn (# i) (synced_list (map snd (Map.elements ms)))) $1
-          * exists l', [[ length l' = Map.cardinal ms - # i ]]
-          * array (LogData xp ^+ i) (List.combine (skipn (# i) (map snd (Map.elements ms))) l') $1
-          * avail_region (LogData xp ^+ $ (Map.cardinal ms)) (# (LogLen xp) - Map.cardinal ms))%pred d' ]]
+          * array (LogData xp ^+ $ (length old)) (firstn (# i) (synced_list (map snd new))) $1
+          * exists l', [[ length l' = length new - # i ]]
+          * array (LogData xp ^+ $ (length old) ^+ i) (List.combine (skipn (# i) (map snd new)) l') $1
+          * avail_region (LogData xp ^+ $ (length old) ^+ $ (length new)) (# (LogLen xp) - length old - length new))%pred d' ]]
     OnCrash crash
     Begin
-      cs <- BUFCACHE.sync_array (LogData xp ^+ i) $0 cs;
+      cs <- BUFCACHE.sync_array (LogData xp ^+ oldlen ^+ i) $0 cs;
       lrx ^(cs)
     Rof ^(cs);
-    rx ^(ms, cs).
+    cs <- BUFCACHE.write (LogHeader xp) (header_to_valu (mk_header (length old + length new))) cs;
+    cs <- BUFCACHE.sync (LogHeader xp) cs;
+    rx ^(cs).
 
-  Definition extend T xp (cs : memstate_cachestate) rx : prog T :=
-    let '^(ms, cs) := mscs in
-    If (lt_dec (wordToNat (LogLen xp)) (Map.cardinal ms)) {
-      rx ^(^(ms, cs), false)
+  Definition extend T xp (cs: cachestate) (old: log_contents) (oldlen: addr) (new: log_contents) rx : prog T :=
+    If (lt_dec (wordToNat (LogLen xp)) (length old + length new)) {
+      rx ^(^(cs), false)
     } else {
       (* Write... *)
-      let^ (ms, cs) <- flush_unsync xp ^(ms, cs);
+      let^ (cs) <- extend_unsync xp cs old oldlen new;
       (* ... and sync *)
-      let^ (ms, cs) <- flush_sync xp ^(ms, cs);
-      rx ^(^(ms, cs), true)
+      let^ (cs) <- extend_sync xp cs old oldlen new;
+      rx ^(^(cs), true)
     }.
-*)
 
   Definition extended_unsynced xp (old: log_contents) (new: log_contents) : @pred addr (@weq addrlen) valuset :=
      ([[ valid_size xp (old ++ new) ]] *
       (LogHeader xp) |=> (header_to_valu (mk_header (length old))) *
-      exists rest others,
+      exists rest rest2,
       (LogDescriptor xp) |-> (descriptor_to_valu (map fst (old ++ new) ++ rest),
-                              map descriptor_to_valu others) *
+                              [descriptor_to_valu (map fst old ++ rest2)]) *
       [[ @Rec.well_formed descriptor_type (map fst (old ++ new) ++ rest) ]] *
-      [[ Forall (@Rec.well_formed descriptor_type) others ]] *
+      [[ @Rec.well_formed descriptor_type (map fst old ++ rest2) ]] *
       array (LogData xp) (synced_list (map snd old)) $1 *
       exists unsynced, (* XXX unsynced is the wrong word for the old values *)
+      [[ length unsynced = length new ]] *
       array (LogData xp ^+ $ (length old)) (List.combine (map snd new) unsynced) $1 *
       avail_region (LogData xp ^+ $ (length old) ^+ $ (length new))
                          (# (LogLen xp) - length old - length new))%pred.
+
+  Lemma in_1 : forall T (x y: T), In x [y] -> x = y.
+    intros.
+    inversion H.
+    congruence.
+    inversion H0.
+  Qed.
+
 
   Theorem extend_unsync_ok : forall xp cs old oldlen new,
     {< F,
@@ -746,6 +757,9 @@ Module DISKLOG.
     solve_lengths.
     rewrite Forall_forall; intuition.
     solve_lengths.
+    rewrite Forall_forall; intuition.
+    solve_lengths.
+
     or_r; cancel.
     unfold valuset_list; simpl; rewrite map_app.
     rewrite <- descriptor_to_valu_zeroes with (n := addr_per_block - length old - length new).
@@ -767,6 +781,10 @@ Module DISKLOG.
     rewrite Forall_forall; intuition.
     unfold upd_prepend.
     solve_lengths.
+    rewrite Forall_forall; intuition.
+    unfold upd_prepend.
+    solve_lengths.
+
     (* step. *)
     eapply pimpl_ok2; [ eauto with prog | ].
     word2nat_clear.
@@ -777,7 +795,6 @@ Module DISKLOG.
     unfold avail_region.
     intuition. pred_apply.
     norm. cancel'. unfold stars; simpl; eapply pimpl_trans; [ apply star_emp_pimpl |].
-    instantiate (others := [_]).
     unfold valuset_list.
     simpl.
     rewrite <- descriptor_to_valu_zeroes with (n := addr_per_block - length old - length new).
@@ -788,19 +805,7 @@ Module DISKLOG.
     unfold valid_size; solve_lengths.
     solve_lengths.
     rewrite Forall_forall; intuition.
-    rewrite Forall_forall; intuition.
-  Lemma in_1 : forall T (x y: T), In x [y] -> x = y.
-    intros.
-    inversion H.
-    congruence.
-    inversion H0.
-  Qed.
-    match goal with
-    | [ H: _ |- _] => apply in_1 in H
-    end.
-    subst.
     solve_lengths.
-    rewrite Forall_forall; intuition.
     congruence.
     congruence.
     autorewrite with lengths in *.
@@ -817,6 +822,8 @@ Module DISKLOG.
     solve_lengths.
     rewrite Forall_forall; intuition.
     solve_lengths.
+    rewrite Forall_forall; intuition.
+    solve_lengths.
     cancel.
     cancel.
     or_r; cancel.
@@ -828,123 +835,376 @@ Module DISKLOG.
     word2nat_clear; autorewrite with lengths in *.
     solve_lengths.
     rewrite Forall_forall; intuition.
+    word2nat_clear; autorewrite with lengths in *.
     solve_lengths.
+    rewrite Forall_forall; intuition.
+    solve_lengths.
+
     Unshelve.
     all: eauto; constructor.
   Qed.
 
-  Hint Extern 1 ({{_}} progseq (flush_unsync _ _) _) => apply flush_unsync_ok : prog.
+  Hint Extern 1 ({{_}} progseq (extend_unsync _ _) _) => apply extend_unsync_ok : prog.
 
-  Theorem flush_sync_ok : forall xp mscs,
-    {< m F,
+
+  Theorem extend_sync_ok : forall xp cs old oldlen new,
+    {< F,
     PRE
+      [[ # oldlen = length old ]] *
       [[ valid_xp xp ]] *
-      let '^(ms, cs) := mscs in
-      exists d, BUFCACHE.rep cs d * 
-      [[ (F * log_rep_unsynced xp m ms)%pred d ]] *
-      [[ Map.cardinal ms <= wordToNat (LogLen xp) ]] *
-      [[ valid_entries m ms ]]
-    POST RET:mscs'
-      let '^(ms, cs) := mscs in
-      let '^(ms', cs') := mscs' in
-      [[ ms = ms' ]] *
-      exists d, BUFCACHE.rep cs' d *
-      [[ (F * log_rep xp m ms')%pred d ]] *
-      [[ Map.cardinal ms' <= wordToNat (LogLen xp) ]]
+      [[ valid_size xp (old ++ new) ]] *
+      exists d, BUFCACHE.rep cs d *
+      [[ (F * extended_unsynced xp old new)%pred d ]]
+    POST RET:^(cs')
+      rep xp F (Synced (old ++ new)) cs'
     CRASH
-      exists mscs' : memstate_cachestate,
-      exists d,
-      let '^(ms, cs) := mscs in
-      (BUFCACHE.rep cs d * [[ (F * log_rep_empty xp)%pred d ]] \/
-       BUFCACHE.rep cs d * [[ (F * log_rep_unsynced xp m ms)%pred d ]])
-    >} flush_sync xp mscs.
+      exists cs' : cachestate,
+      rep xp F (ExtendedDescriptor old) cs' \/ rep xp F (Synced old) cs' \/ rep xp F (Extended old new) cs' \/ rep xp F (Synced (old ++ new)) cs'
+    >} extend_sync xp cs old oldlen new.
   Proof.
-    unfold flush_sync; log_unfold; unfold avail_region, memstate_cachestate.
-    destruct mscs as [ms cs].
+    unfold extend_sync; disklog_unfold; unfold avail_region, extended_unsynced.
     intros.
     solve_lengths_prepare.
-    step.
-    step.
-
-    ring_simplify (LogData xp ^+ $0).
-    cancel; eauto.
-    omega.
-
-    step.
-    instantiate (1 := List.combine (skipn # m1 (map snd (Map.elements ms))) l4).
+    (* step. (* XXX takes a very long time *) *)
+    eapply pimpl_ok2; [ eauto with prog | ].
     cancel.
-    solve_lengths.
-
-    step.
-    try_arrays_lengths.
-    split_lists.
-    rewrite skipn_skipn.
-    rewrite (plus_comm 1).
+    eapply pimpl_ok2; [ eauto with prog | ].
+    unfold avail_region.
+    cancel.
+    word2nat_clear; word2nat_auto.
     rewrite Nat.add_0_r.
-    erewrite firstn_plusone_selN.
-    rewrite <- app_assoc.
+    fold unifiable_array; cancel.
+    solve_lengths.
+    solve_lengths.
+    eapply pimpl_ok2; [ eauto with prog | ].
+    cancel.
+    word2nat_clear; word2nat_auto.
+    fold unifiable_array; cancel.
+    solve_lengths.
+    unfold valid_size in *.
+    eapply pimpl_ok2; [ eauto with prog | ].
+    cancel.
+    word2nat_clear.
+    autorewrite with lengths in *.
+    word2nat_auto.
+    array_match_prepare.
+    repeat chop_shortest_suffix.
+    auto.
+    (* subst_evars here would cause an anomaly trying to instantiate H14 *)
+    subst H14.
     reflexivity.
+    auto.
+    subst_evars; reflexivity.
+    subst H14.
     solve_lengths.
-    erewrite firstn_plusone_selN.
+    (* XXX revise once the anomalies are fixed *)
+    subst H14 H19.
+    erewrite firstn_plusone_selN by solve_lengths.
+    trivial.
+    trivial.
+    subst H12; trivial.
+    subst H11.
+    solve_lengths.
+    unfold upd_sync.
+    subst H11 H12.
+    unfold sel, upd; simpl.
+    instantiate (l'0 := skipn 1 l').
+    subst H4.
+    repeat rewrite selN_combine.
+    lists_eq.
+    subst H6.
+    trivial.
+    solve_lengths.
+    autorewrite with lengths in *.
+    solve_lengths.
+    solve_lengths.
+    cancel.
+    or_r; or_l. norm. cancel'.
+    repeat constructor. pred_apply.
+
+    rewrite map_app.
     rewrite <- app_assoc.
-    rewrite repeat_selN.
+    cancel.
+    word2nat_clear.
+    unfold valid_size in *.
+    autorewrite with lengths in *.
+    array_match.
+    unfold synced_list. autorewrite with lengths. trivial.
+    word2nat_clear.
+    unfold valid_size in *.
+    autorewrite with lengths in *.
+    solve_lengths.
+    word2nat_clear.
+    unfold valid_size in *.
+    autorewrite with lengths in *.
+    solve_lengths.
+    rewrite Forall_forall; intuition.
+    word2nat_clear.
+    unfold valid_size in *.
+    autorewrite with lengths in *.
+    solve_lengths.
+    solve_lengths.
+
+    or_r; or_l; cancel.
+    rewrite map_app.
+    rewrite <- app_assoc.
+    cancel.
+    word2nat_clear.
+    unfold valid_size in *.
+    autorewrite with lengths in *.
+    array_match.
+    unfold synced_list. autorewrite with lengths. trivial.
+    word2nat_clear.
+    unfold valid_size in *.
+    autorewrite with lengths in *.
+    solve_lengths.
+    word2nat_clear.
+    unfold valid_size in *.
+    autorewrite with lengths in *.
+    unfold upd_sync.
+    solve_lengths.
+    unfold upd_sync.
+    solve_lengths.
+    word2nat_clear.
+    unfold valid_size in *.
+    autorewrite with lengths in *.
+    solve_lengths.
+    word2nat_clear.
+    unfold valid_size in *.
+    autorewrite with lengths in *.
+    solve_lengths.
+    rewrite Forall_forall; intuition.
+    word2nat_clear.
+    unfold valid_size in *.
+    autorewrite with lengths in *.
+    unfold upd_sync.
+    solve_lengths.
+
+    eapply pimpl_ok2; [ eauto with prog | ].
+    cancel.
+    eapply pimpl_ok2; [ eauto with prog | ].
+    cancel.
+    eapply pimpl_ok2; [ eauto with prog | ].
+    cancel.
+    word2nat_clear.
+    autorewrite with lengths in *.
+    rewrite map_app.
+    cancel.
+    unfold synced_list.
+    array_match_prepare.
+    repeat chop_shortest_suffix.
+    auto.
+    subst_evars.
     reflexivity.
-
+    reflexivity.
+    subst H6. (* subst_evars here leads to an anomaly *)
+    reflexivity.
+    subst H4.
     solve_lengths.
-    solve_lengths.
-    solve_lengths.
-    solve_lengths.
-    solve_lengths.
-    solve_lengths.
-    solve_lengths.
-    solve_lengths.
-
-    or_l. cancel.
-    try_arrays_lengths.
-    solve_lengths.
-
-    or_l. cancel.
-    try_arrays_lengths.
-    unfold upd_sync; solve_lengths.
-    unfold upd_sync; solve_lengths.
-    unfold upd_sync; solve_lengths.
-
-    step.
-    try_arrays_lengths.
-    rewrite firstn_oob by solve_lengths.
-    eauto.
-    solve_lengths.
-    solve_lengths.
+    subst H4 H6.
+    unfold valid_size in *.
+    autorewrite with lengths in *.
+    lists_eq.
+    trivial.
+    rewrite app_repeat.
+    trivial.
+    subst_evars.
+    trivial.
+    word2nat_clear.
+    unfold valid_size in *.
+    autorewrite with lengths in *.
     solve_lengths.
 
-    or_r. cancel.
-    try_arrays_lengths.
-    solve_lengths.
-    solve_lengths.
+    cancel.
+    or_r; or_r; or_l; cancel.
+    word2nat_clear. unfold valid_size in *. autorewrite with lengths in *.
+    unfold synced_list.
+    array_match_prepare.
+    repeat chop_shortest_suffix.
+    auto.
+    subst_evars. reflexivity.
+    reflexivity.
+    (* subst_evars here gives an anomaly *) subst H6. reflexivity.
+    subst H4. solve_lengths.
+    subst H4 H6. lists_eq.
+    trivial.
+    rewrite app_repeat. trivial.
+    subst H1. reflexivity.
+    word2nat_clear. unfold valid_size in *. autorewrite with lengths in *.
     solve_lengths.
 
-    or_l. cancel.
-    try_arrays_lengths.
+    or_r; or_r; or_r; cancel.
+    word2nat_clear. unfold valid_size in *. autorewrite with lengths in *.
+    unfold synced_list.
+    cancel.
+    array_match_prepare.
+    repeat chop_shortest_suffix.
+    auto.
+    subst_evars. reflexivity.
+    reflexivity.
+    (* subst_evars here gives an anomaly *) subst H6. reflexivity.
+    subst H4. solve_lengths.
+    subst H4 H6. lists_eq.
+    trivial.
+    rewrite app_repeat. trivial.
+    subst H1. reflexivity.
+    word2nat_clear. unfold valid_size in *. autorewrite with lengths in *.
+    solve_lengths.
+
+    cancel.
+    or_r; or_l; cancel.
+    rewrite map_app.
+    rewrite <- app_assoc.
+    cancel.
+    word2nat_clear.
+    unfold valid_size in *.
+    autorewrite with lengths in *.
+    array_match.
+    unfold synced_list. autorewrite with lengths. trivial.
+    word2nat_clear.
+    unfold valid_size in *.
+    autorewrite with lengths in *.
+    solve_lengths.
+    word2nat_clear.
+    unfold valid_size in *.
+    autorewrite with lengths in *.
+    unfold upd_sync.
+    solve_lengths.
+    unfold upd_sync.
+    solve_lengths.
+    word2nat_clear.
+    unfold valid_size in *.
+    autorewrite with lengths in *.
+    solve_lengths.
+    word2nat_clear.
+    unfold valid_size in *.
+    autorewrite with lengths in *.
+    solve_lengths.
+    rewrite Forall_forall; intuition.
+    word2nat_clear.
+    unfold valid_size in *.
+    autorewrite with lengths in *.
+    unfold upd_sync.
+    solve_lengths.
+    word2nat_clear.
+    unfold valid_size in *.
+    autorewrite with lengths in *.
+    unfold upd_sync.
+    solve_lengths.
+
+    cancel.
+    or_r; or_r; or_l; cancel.
+    word2nat_clear.
+    unfold valid_size in *.
+    autorewrite with lengths in *.
+    unfold synced_list.
+    array_match_prepare.
+    repeat chop_shortest_suffix.
+    auto.
+    subst_evars. reflexivity.
+    reflexivity.
+    (* subst_evars here gives an anomaly *) subst H6. reflexivity.
+    subst H4. solve_lengths.
+    subst H4 H6. lists_eq.
+    trivial.
+    rewrite app_repeat. trivial.
+    subst H1. reflexivity.
+    word2nat_clear. unfold valid_size in *. autorewrite with lengths in *.
+    solve_lengths.
+
+    cancel.
+    or_r; or_l; cancel.
+    instantiate (1 := d').
+    pred_apply. cancel.
+    rewrite map_app.
+    rewrite <- app_assoc.
+    cancel.
+    word2nat_clear.
+    unfold valid_size in *.
+    autorewrite with lengths in *.
+    array_match.
+    unfold synced_list. autorewrite with lengths. trivial.
+    word2nat_clear.
+    unfold valid_size in *.
+    autorewrite with lengths in *.
+    solve_lengths.
+    word2nat_clear.
+    unfold valid_size in *.
+    autorewrite with lengths in *.
+    unfold upd_sync.
+    solve_lengths.
+    unfold upd_sync.
+    solve_lengths.
+    word2nat_clear.
+    unfold valid_size in *.
+    autorewrite with lengths in *.
+    solve_lengths.
+    word2nat_clear.
+    unfold valid_size in *.
+    autorewrite with lengths in *.
+    solve_lengths.
+    rewrite Forall_forall; intuition.
+    word2nat_clear.
+    unfold valid_size in *.
+    autorewrite with lengths in *.
+    unfold upd_sync.
+    solve_lengths.
+
+    cancel.
+    rewrite map_app.
+    rewrite <- app_assoc.
+    word2nat_clear.
+    unfold valid_size in *.
+    autorewrite with lengths in *.
+    cancel.
+    array_match.
+    unfold synced_list. autorewrite with lengths. trivial.
+    word2nat_clear.
+    unfold valid_size in *.
+    autorewrite with lengths in *.
+    solve_lengths.
+    word2nat_clear.
+    unfold valid_size in *.
+    autorewrite with lengths in *.
+    unfold upd_sync.
+    solve_lengths.
+    unfold upd_sync.
+    solve_lengths.
+    word2nat_clear.
+    unfold valid_size in *.
+    autorewrite with lengths in *.
+    solve_lengths.
+    word2nat_clear.
+    unfold valid_size in *.
+    autorewrite with lengths in *.
+    solve_lengths.
+    rewrite Forall_forall; intuition.
+    word2nat_clear.
+    unfold valid_size in *.
+    autorewrite with lengths in *.
+    unfold upd_sync.
     solve_lengths.
 
     Unshelve.
     all: auto.
   Qed.
 
-  Hint Extern 1 ({{_}} progseq (flush_sync _ _) _) => apply flush_sync_ok : prog.
 
-  Theorem flush_ok : forall xp mscs,
-    {< m1 m2 F,
+  Hint Extern 1 ({{_}} progseq (extend_sync _ _) _) => apply extend_sync_ok : prog.
+
+  Theorem extend_ok : forall xp cs old new rx,
+    {< F,
     PRE
-      rep xp F (ActiveTxn m1 m2) mscs
-    POST RET:^(mscs,r)
-      ([[ r = true ]] * rep xp F (FlushedTxn m1 m2) mscs) \/
-      ([[ r = false ]] * rep xp F (ActiveTxn m1 m2) mscs)
+      rep xp F (Synced old) cs
+    POST RET:^(cs,r)
+      ([[ r = true ]] * rep xp F (Synced new) cs \/
+      ([[ r = false ]] * rep xp F (Synced old) cs
     CRASH
-      exists mscs', rep xp F (ActiveTxn m1 m2) mscs' \/ rep xp F (FlushedUnsyncTxn m1 m2) mscs'
-    >} flush xp mscs.
+      exists cs' : cachestate,
+      rep xp F (ExtendedDescriptor old) cs' \/ rep xp F (Synced old) cs' \/ rep xp F (Extended old new) cs' \/ rep xp F (Synced (old ++ new)) cs'
+    >} extend xp old new cs.
   Proof.
-    unfold flush, rep, rep_inner.
+    unfold extend.
     step.
     step.
     step.
